theories/lifetime/model/definitions.v
@@ -212,10 +212,10 @@ Notation "q .[ κ ]" := (lft_tok q κ)
     (format "q .[ κ ]", at level 0) : uPred_scope.
 Notation "[† κ ]" := (lft_dead κ) (format "[† κ ]"): uPred_scope.
 
-Notation "&{ κ } P" := (bor κ P)
-  (format "&{ κ }  P", at level 20, right associativity) : uPred_scope.
-Notation "&{ κ , i } P" := (idx_bor κ i P)
-  (format "&{ κ , i }  P", at level 20, right associativity) : uPred_scope.
+Notation "&{ κ }" := (bor κ)
+  (format "&{ κ }", at level 20, right associativity) : uPred_scope.
+Notation "&{ κ , i }" := (idx_bor κ i)
+  (format "&{ κ , i }", at level 20, right associativity) : uPred_scope.
 
 Infix "⊑" := lft_incl (at level 70) : uPred_scope.
 
